Add draft statement of theorem for `CONSTAINTS` program

Is0/Programs.lean
@@ -15,30 +15,30 @@ def is0OriginalProgram (x : Felt) (y : Felt) (z : Felt) : State × Option Prop :
               , buffers := Map.fromList [("in", [x]), ("out", [y, z])]
               , constraints := []
               }
-    (.Sequence
+  (.Sequence
     (.Assign "1" (Op.Const 1))
-    (.Sequence
+  (.Sequence
     (.Assign "x" (Op.Get ⟨"in"⟩ 0 0))
-    (.Sequence
+  (.Sequence
     (.Assign "isZeroBit" (Op.Isz ⟨"x"⟩))
-    (.Sequence
+  (.Sequence
     (.Set ⟨"out"⟩ 0 ⟨"isZeroBit"⟩)
-    (.Sequence
+  (.Sequence
     (.Assign "invVal" (Op.Inv ⟨"x"⟩))
-    (.Sequence
+  (.Sequence
     (.Set ⟨"out"⟩ 1 ⟨"invVal"⟩)
-    (.Sequence
+  (.Sequence
     (.Assign "out[0]" (Op.Get ⟨"out"⟩ 0 0))
-    (.Sequence
+  (.Sequence
     (.If ⟨"out[0]"⟩
       (.Eqz ⟨"x"⟩))
-    (.Sequence
+  (.Sequence
     (.Assign "1 - out[0]" (Op.Sub ⟨"1"⟩ ⟨"out[0]"⟩))
     (.If ⟨"1 - out[0]"⟩
       (.Sequence
-      (.Assign "out[1]" (Op.Get ⟨"out"⟩ 1 0))
+        (.Assign "out[1]" (Op.Get ⟨"out"⟩ 1 0))
       (.Sequence
-      (.Assign "x * out[1]" (Op.Mul ⟨"x"⟩ ⟨"out[1]"⟩))
+        (.Assign "x * out[1]" (Op.Mul ⟨"x"⟩ ⟨"out[1]"⟩))
       (.Sequence
         (.Assign "x * out[1] - 1" (Op.Sub ⟨"x * out[1]"⟩ ⟨"1"⟩))
         (.Eqz ⟨"x * out[1] - 1"⟩))))))))))))))
@@ -51,33 +51,33 @@ def is0ConstraintsProgram (x : Felt) (y : Felt) (z : Felt) : State × Option Pro
               , constraints := []
               }
   (.Sequence
-    (.Sequence
-      (.Sequence
-        (.Sequence
-          (.Sequence
-            (.Sequence
-              (.Sequence
-                (.Sequence
-                  (.Sequence
-                    (.Sequence
-                      (.Sequence
-                        (.Sequence
-                          (.Assign "1" (Op.Const 1))
-                          (.Assign "true" Op.True))
-                          (.Assign "x" (Op.Get ⟨"in"⟩ 0 0)))
-                          (.Assign "isZeroBit" (Op.Get ⟨"out"⟩ 0 0)))
-                          (.Assign "x = 0" (Op.AndEqz ⟨"true"⟩ ⟨"x"⟩)))
-                          (.Assign "IF isZeroBit THEN (x = 0) ELSE true" (Op.AndCond ⟨"true"⟩ ⟨"isZeroBit"⟩ ⟨"x = 0"⟩)))
-                          (.Assign "1 - isZeroBit" (Op.Sub ⟨"1"⟩ ⟨"isZeroBit"⟩)))
-                          (.Assign "invVal" (Op.Get ⟨"out"⟩ 1 0)))
-                          (.Assign "x * invVal" (Op.Mul ⟨"x"⟩ ⟨"invVal"⟩)))
-                          (.Assign "x * invVal - 1" (Op.Sub ⟨"x * invVal"⟩ ⟨"1"⟩)))
-                          (.Assign "x * invVal - 1 = 0" (Op.AndEqz ⟨"true"⟩ ⟨"x * invVal - 1"⟩)))
-                          (.Assign "result"
-                            (Op.AndCond
-                              ⟨"IF isZeroBit THEN (x = 0) ELSE true"⟩
-                              ⟨"1 - isZeroBit"⟩
-                              ⟨"x * invVal - 1 = 0"⟩)))
-                          (.Return "result"))
+    (.Assign "1" (Op.Const 1))
+  (.Sequence
+    (.Assign "true" Op.True)
+  (.Sequence
+    (.Assign "x" (Op.Get ⟨"in"⟩ 0 0))
+  (.Sequence
+    (.Assign "isZeroBit" (Op.Get ⟨"out"⟩ 0 0))
+  (.Sequence
+    (.Assign "x = 0" (Op.AndEqz ⟨"true"⟩ ⟨"x"⟩))
+  (.Sequence
+    (.Assign "IF isZeroBit THEN (x = 0) ELSE true" (Op.AndCond ⟨"true"⟩ ⟨"isZeroBit"⟩ ⟨"x = 0"⟩))
+  (.Sequence
+    (.Assign "1 - isZeroBit" (Op.Sub ⟨"1"⟩ ⟨"isZeroBit"⟩))
+  (.Sequence
+    (.Assign "invVal" (Op.Get ⟨"out"⟩ 1 0))
+  (.Sequence
+    (.Assign "x * invVal" (Op.Mul ⟨"x"⟩ ⟨"invVal"⟩))
+  (.Sequence
+    (.Assign "x * invVal - 1" (Op.Sub ⟨"x * invVal"⟩ ⟨"1"⟩))
+  (.Sequence
+    (.Assign "x * invVal - 1 = 0" (Op.AndEqz ⟨"true"⟩ ⟨"x * invVal - 1"⟩))
+  (.Sequence
+    (.Assign "result"
+      (Op.AndCond
+        ⟨"IF isZeroBit THEN (x = 0) ELSE true"⟩
+        ⟨"1 - isZeroBit"⟩
+        ⟨"x * invVal - 1 = 0"⟩))
+    (.Return "result")))))))))))))
 
 end Risc0
