Is0/Is0.lean
@@ -10,10 +10,11 @@ import Is0.Programs
 
 namespace Risc0
 
-theorem is0OriginalProgram_constraints_are_what_we_expect :
-  ∀ x y z : Felt, (is0OriginalProgram x y z).1.constraints.foldr And _root_.True ↔ (if x == 0 then x = 0 else x * x⁻¹ - 1 = 0) := by
+-- Looks like we need to give `y` and `z` some meaning in this case.
+theorem is0ConstraintsProgram_constraints_are_what_we_expect {result : Prop} :
+  ∀ x y z : Felt, (is0ConstraintsProgram x y z).2 = some (if x == 0 then x = 0 else x * x⁻¹ - 1 = 0) := by
   intros x y z
-  unfold is0OriginalProgram
+  unfold is0ConstraintsProgram
   by_cases x = 0
   rw [h]
   rw [Cirgen.step_Sequence_Assign_collapsible]
@@ -29,55 +30,43 @@ theorem is0OriginalProgram_constraints_are_what_we_expect :
   simp only [State.update, Map.empty, Map.fromList, Map.update, beq_iff_eq, ne_eq]
   unfold Op.eval ; simp only
   simp only [beq_iff_eq, ne_eq]
-  rw [if_neg h]
-  rw [if_neg h]
-  rw [Cirgen.step_Sequence_Set_collapsible [y, z] 0]
-  simp only [Map.update, beq_iff_eq, ne_eq]
   rw [Cirgen.step_Sequence_Assign_collapsible]
-  simp only [State.update, Map.update, beq_iff_eq, ne_eq]
+  simp only [State.update, Map.empty, Map.fromList, Map.update, beq_iff_eq, ne_eq]
   unfold Op.eval ; simp only
-  unfold List.set
-  simp only [beq_iff_eq, ne_eq]
-  rw [if_neg h]
-  rw [Cirgen.step_Sequence_Set_collapsible [0, z] x⁻¹]
-  simp only [Map.update, beq_iff_eq, List.set_succ, and_true, ne_eq]
+  simp only [beq_iff_eq, ite_self]
   rw [Cirgen.step_Sequence_Assign_collapsible]
-  simp only [State.update, Map.empty, Map.fromList, Map.update, beq_iff_eq, and_true, ne_eq]
+  simp only [State.update, Map.empty, Map.fromList, Map.update, beq_iff_eq, ne_eq]
   unfold Op.eval ; simp only
-  unfold List.getD ; unfold List.get? ; unfold Option.getD ; simp only
-  rw [Cirgen.step_Sequence_If_collapsible 0]
-  unfold List.set
-  simp only [and_true, ne_eq]
+  simp only [beq_iff_eq, ite_self]
   rw [Cirgen.step_Sequence_Assign_collapsible]
+  simp only [State.update, Map.empty, Map.fromList, Map.update, beq_iff_eq, ne_eq]
   unfold Op.eval ; simp only
-  simp only [State.update, Map.update, beq_iff_eq, sub_zero, and_true, ne_eq]
-  rw [ite_true]
-  rw [Cirgen.step_If_collapsible 1]
-  simp only [List.foldr, and_true, ne_eq]
+  simp only [beq_iff_eq, ite_self]
+  rw [Cirgen.step_Sequence_Assign_collapsible]
+  simp only [State.update, Map.empty, Map.fromList, Map.update, beq_iff_eq, ne_eq]
+  unfold Op.eval ; simp only
+  simp only [beq_iff_eq, ite_self]
+  rw [Cirgen.step_Sequence_Assign_collapsible]
+  simp only [State.update, Map.empty, Map.fromList, Map.update, beq_iff_eq, ne_eq]
+  unfold List.getD ; unfold Option.getD ; unfold List.get? ; unfold List.get?; simp only
+  unfold Op.eval ; simp only
+  simp only [beq_iff_eq, ite_self]
+  rw [Cirgen.step_Sequence_Assign_collapsible]
+  simp only [State.update, Map.empty, Map.fromList, Map.update, beq_iff_eq, ne_eq]
+  unfold Op.eval ; simp only
+  simp only [beq_iff_eq, ite_self]
+  rw [Cirgen.step_Sequence_Assign_collapsible]
+  simp only [State.update, Map.empty, Map.fromList, Map.update, beq_iff_eq, ne_eq]
+  unfold Op.eval ; simp only
+  simp only [beq_iff_eq, ite_self]
+  unfold Cirgen.step
+  nth_rewrite 1 [Cirgen.step]
   nth_rewrite 1 [Op.assign]
   nth_rewrite 1 [Op.eval]
-  simp only [Map.update, ite_true, Option.some.injEq, ne_eq]
-  nth_rewrite 1 [Op.assign]
-  nth_rewrite 1 [Op.eval]
-  simp only [ite_true, ite_false, List.getD_cons_succ, List.getD_cons_zero, Map.update, beq_iff_eq, Option.some.injEq, ne_eq]
-  nth_rewrite 1 [Op.assign]
-  nth_rewrite 1 [Op.eval]
-  simp only [ite_true, ite_false, List.getD_cons_succ, List.getD_cons_zero, Map.update, beq_iff_eq, ne_eq, Option.some.injEq]
-  nth_rewrite 1 [Op.assign]
-  nth_rewrite 1 [Op.eval]
-  simp only [ne_eq, Map.update, ite_false, Option.some.injEq]
-  nth_rewrite 1 [Op.assign]
-  nth_rewrite 1 [Op.eval]
-  simp only [ne_eq, ite_true, ite_false, List.getD_cons_succ, List.getD_cons_zero, Map.update, beq_iff_eq, ite_self]
-  simp only [ite_false, ite_true]
-  simp only [ite_false, ite_true]
-  apply @hab x y z
-  rw [Cirgen.step_Eqz_collapsible x]
-  simp only [ne_eq, Prod.mk.injEq, State.mk.injEq, and_false, and_true, not_false_iff]
-  simp only [ite_false, ite_true]
-  simp only [ite_false, ite_true]
-  simp only [ite_false, ite_true]
-  simp only [ite_false, ite_true]
-  simp only [ite_false, ite_true]
+  simp only [zero_mul, zero_sub, neg_eq_zero, and_false, ite_false, ite_true, beq_iff_eq, Map.update]
+  nth_rewrite 1 [Cirgen.step]
+  simp only [ite_false, ite_true, Option.some.injEq, ite_eq_left_iff]
+  sorry
+  sorry
 
 end Risc0
